<?xml version="1.0"?>


<!DOCTYPE rdf:RDF [
    <!ENTITY dcterms "http://purl.org/dc/terms/" >
    <!ENTITY owl "http://www.w3.org/2002/07/owl#" >
    <!ENTITY obo "http://purl.obolibrary.org/obo/" >
    <!ENTITY dc "http://purl.org/dc/elements/1.1/" >
    <!ENTITY xsd "http://www.w3.org/2001/XMLSchema#" >
    <!ENTITY rdfs "http://www.w3.org/2000/01/rdf-schema#" >
    <!ENTITY rdf "http://www.w3.org/1999/02/22-rdf-syntax-ns#" >
    <!ENTITY tc "http://rs.tdwg.org/ontology/voc/TaxonConcept#" >
]>


<rdf:RDF xmlns="http://phylotastic.org/terms/tnrs.rdf#"
     xml:base="http://phylotastic.org/terms/tnrs.rdf"
     xmlns:dc="http://purl.org/dc/elements/1.1/"
     xmlns:obo="http://purl.obolibrary.org/obo/"
     xmlns:rdfs="http://www.w3.org/2000/01/rdf-schema#"
     xmlns:tc="http://rs.tdwg.org/ontology/voc/TaxonConcept#"
     xmlns:owl="http://www.w3.org/2002/07/owl#"
     xmlns:xsd="http://www.w3.org/2001/XMLSchema#"
     xmlns:rdf="http://www.w3.org/1999/02/22-rdf-syntax-ns#"
     xmlns:dcterms="http://purl.org/dc/terms/">
    <owl:Ontology rdf:about="http://phylotastic.org/terms/tnrs.rdf">
        <dc:title>Taxonomic Name Resolution Service (TNRS) result ontology and data model</dc:title>
        <rdfs:comment>When you use this ontology in your work, please give credit to the extent possible, for example by referring to the canonical URI of the ontology. To cite the ontology in a scientific publication, for the time being please use the following article.

Stoltzfus A. et al. 2013. Phylotastic! Making Tree-of-life Knowledge Accessible, Reusable and Convenient. BMC Bioinformatics. Vol. 14. doi:10.1186/1471-2105-14-158.</rdfs:comment>
        <dc:creator>Hilmar Lapp</dc:creator>
        <dc:rights>http://creativecommons.org/publicdomain/zero/1.0/</dc:rights>
        <rdfs:comment>The source code repository for this ontology is at http://github.com/phylotastic/ontologies/tnrs.</rdfs:comment>
        <dc:description>The TNRS ontology is intended as a shared vocabulary and RDF data model for representing the results from Taxonomic Name Resolution Service (TNRS) requests, and for storing them in a triple store. It was initially created in June 2012 at the first of the Phylotastic hackathon series organized and run by the Hackathons, Interoperability, Phylogenetics (HIP) Working Group at the National Evolutionary Synthesis Center (NESCent). 

The ontology subsequently underwent a few refinements, mostly to draw more from existing vocabularies where possible, and to do so consistent with the semantics of those vocabularies.

The source repository where the ontology is maintained includes instance documents (in RDF/XML and quite readable Turtle versions) as examples, and visual renderings of the corresponding RDF graphs. These instance documents are based off of the example on the TNRS wiki page (http://www.evoio.org/wiki/Phylotastic/TNRS).

The primary reason that the canonical URI of the ontology ends in .rdf is so that Github serves it under the correct mimetype.
</dc:description>
        <owl:versionIRI rdf:resource="http://phylotastic.org/terms/2013-06/tnrs.rdf"/>
        <owl:imports rdf:resource="http://rs.tdwg.org/ontology/voc/TaxonConcept"/>
    </owl:Ontology>
    


    <!-- 
    ///////////////////////////////////////////////////////////////////////////////////////
    //
    // Annotation properties
    //
    ///////////////////////////////////////////////////////////////////////////////////////
     -->

    <owl:AnnotationProperty rdf:about="&dc;rights"/>
    


    <!-- 
    ///////////////////////////////////////////////////////////////////////////////////////
    //
    // Datatypes
    //
    ///////////////////////////////////////////////////////////////////////////////////////
     -->

    


    <!-- 
    ///////////////////////////////////////////////////////////////////////////////////////
    //
    // Object Properties
    //
    ///////////////////////////////////////////////////////////////////////////////////////
     -->

    


    <!-- http://phylotastic.org/terms/tnrs.rdf#matches -->

    <owl:ObjectProperty rdf:about="http://phylotastic.org/terms/tnrs.rdf#matches">
        <rdfs:label>matches</rdfs:label>
        <rdfs:comment>The relationship between a taxonomic name resolution request for a name and the resulting matches.</rdfs:comment>
        <rdfs:range rdf:resource="http://phylotastic.org/terms/tnrs.rdf#Match"/>
        <rdfs:domain rdf:resource="http://phylotastic.org/terms/tnrs.rdf#NameResolution"/>
    </owl:ObjectProperty>
    


    <!-- http://phylotastic.org/terms/tnrs.rdf#resolvesAs -->

    <owl:ObjectProperty rdf:about="http://phylotastic.org/terms/tnrs.rdf#resolvesAs">
        <rdfs:label>resolvesAs</rdfs:label>
        <rdfs:comment>The relationship between a taxonomic unit or entity and its taxonomic name resolution.</rdfs:comment>
        <rdfs:range rdf:resource="http://phylotastic.org/terms/tnrs.rdf#NameResolution"/>
        <rdfs:domain rdf:resource="&obo;CDAO_0000138"/>
    </owl:ObjectProperty>
    


    <!-- http://phylotastic.org/terms/tnrs.rdf#usedSource -->

    <owl:ObjectProperty rdf:about="http://phylotastic.org/terms/tnrs.rdf#usedSource">
        <rdfs:label>usedSource</rdfs:label>
        <rdfs:comment>The relationship between a TNRS resolution request and the resolution sources used by the TNRS in carrying out the request.</rdfs:comment>
        <rdfs:range rdf:resource="http://phylotastic.org/terms/tnrs.rdf#ResolutionSource"/>
    </owl:ObjectProperty>
    


    <!-- http://purl.org/dc/terms/references -->

    <owl:ObjectProperty rdf:about="&dcterms;references"/>
    


    <!-- http://purl.org/dc/terms/source -->

    <owl:ObjectProperty rdf:about="&dcterms;source"/>
    


    <!-- 
    ///////////////////////////////////////////////////////////////////////////////////////
    //
    // Data properties
    //
    ///////////////////////////////////////////////////////////////////////////////////////
     -->

    


    <!-- http://phylotastic.org/terms/tnrs.rdf#acceptedName -->

    <owl:DatatypeProperty rdf:about="http://phylotastic.org/terms/tnrs.rdf#acceptedName">
        <rdfs:label>acceptedName</rdfs:label>
        <rdfs:comment>The taxonomic name reported as accepted name by the TNRS source reporting a match to a query.</rdfs:comment>
    </owl:DatatypeProperty>
    


    <!-- http://phylotastic.org/terms/tnrs.rdf#hasRank -->

    <owl:DatatypeProperty rdf:about="http://phylotastic.org/terms/tnrs.rdf#hasRank">
        <rdfs:label>hasRank</rdfs:label>
        <rdfs:comment>The suggested rank of a TNRS source among the sources a TNRS queries.</rdfs:comment>
    </owl:DatatypeProperty>
    


    <!-- http://phylotastic.org/terms/tnrs.rdf#matchCount -->

    <owl:DatatypeProperty rdf:about="http://phylotastic.org/terms/tnrs.rdf#matchCount">
        <rdfs:label>matchCount</rdfs:label>
        <rdfs:comment>The number of matches obtained from the TNRS query for a submitted name.</rdfs:comment>
    </owl:DatatypeProperty>
    


    <!-- http://phylotastic.org/terms/tnrs.rdf#matchedName -->

    <owl:DatatypeProperty rdf:about="http://phylotastic.org/terms/tnrs.rdf#matchedName">
        <rdfs:label>matchedName</rdfs:label>
        <rdfs:comment>The taxonomic name matched by a TNRS source.</rdfs:comment>
    </owl:DatatypeProperty>
    


    <!-- http://phylotastic.org/terms/tnrs.rdf#score -->

    <owl:DatatypeProperty rdf:about="http://phylotastic.org/terms/tnrs.rdf#score">
        <rdfs:label>score</rdfs:label>
        <rdfs:comment>The score of a match reported by a TNRS source.</rdfs:comment>
    </owl:DatatypeProperty>
    


    <!-- http://phylotastic.org/terms/tnrs.rdf#sourceStatus -->

    <owl:DatatypeProperty rdf:about="http://phylotastic.org/terms/tnrs.rdf#sourceStatus">
        <rdfs:label>sourceStatus</rdfs:label>
        <rdfs:comment>The status of a TNRS source at the time the request was made. TNRS sources with &quot;offline&quot; or &quot;temporarily offline&quot; status may NOT have been queried, and their results may be missing from the resolution document.</rdfs:comment>
    </owl:DatatypeProperty>
    


    <!-- http://phylotastic.org/terms/tnrs.rdf#submitDate -->

    <owl:DatatypeProperty rdf:about="http://phylotastic.org/terms/tnrs.rdf#submitDate">
        <rdfs:label>submitDate</rdfs:label>
        <rdfs:comment>The date and time that the TNRS resolution job was submitted, in ISO 8601 format.</rdfs:comment>
    </owl:DatatypeProperty>
    


    <!-- http://phylotastic.org/terms/tnrs.rdf#submittedName -->

    <owl:DatatypeProperty rdf:about="http://phylotastic.org/terms/tnrs.rdf#submittedName">
        <rdfs:label>submittedName</rdfs:label>
        <rdfs:comment>The name that was submitted to the TNRS for resolution.</rdfs:comment>
    </owl:DatatypeProperty>
    


    <!-- http://purl.org/dc/elements/1.1/title -->

    <owl:DatatypeProperty rdf:about="&dc;title"/>
    


    <!-- 
    ///////////////////////////////////////////////////////////////////////////////////////
    //
    // Classes
    //
    ///////////////////////////////////////////////////////////////////////////////////////
     -->

    


    <!-- http://phylotastic.org/terms/tnrs.rdf#Match -->

    <owl:Class rdf:about="http://phylotastic.org/terms/tnrs.rdf#Match">
        <rdfs:label>Match</rdfs:label>
        <owl:equivalentClass>
            <owl:Class>
                <owl:intersectionOf rdf:parseType="Collection">
                    <owl:Restriction>
                        <owl:onProperty rdf:resource="http://phylotastic.org/terms/tnrs.rdf#usedSource"/>
                        <owl:onClass rdf:resource="http://phylotastic.org/terms/tnrs.rdf#ResolutionSource"/>
                        <owl:qualifiedCardinality rdf:datatype="&xsd;nonNegativeInteger">1</owl:qualifiedCardinality>
                    </owl:Restriction>
                    <owl:Restriction>
                        <owl:onProperty rdf:resource="&tc;toTaxon"/>
                        <owl:onClass rdf:resource="&tc;TaxonConcept"/>
                        <owl:qualifiedCardinality rdf:datatype="&xsd;nonNegativeInteger">1</owl:qualifiedCardinality>
                    </owl:Restriction>
                    <owl:Restriction>
                        <owl:onProperty rdf:resource="http://phylotastic.org/terms/tnrs.rdf#acceptedName"/>
                        <owl:qualifiedCardinality rdf:datatype="&xsd;nonNegativeInteger">1</owl:qualifiedCardinality>
                        <owl:onDataRange rdf:resource="&xsd;string"/>
                    </owl:Restriction>
                    <owl:Restriction>
                        <owl:onProperty rdf:resource="http://phylotastic.org/terms/tnrs.rdf#matchedName"/>
                        <owl:qualifiedCardinality rdf:datatype="&xsd;nonNegativeInteger">1</owl:qualifiedCardinality>
                        <owl:onDataRange rdf:resource="&xsd;string"/>
                    </owl:Restriction>
                    <owl:Restriction>
                        <owl:onProperty rdf:resource="http://phylotastic.org/terms/tnrs.rdf#score"/>
                        <owl:maxQualifiedCardinality rdf:datatype="&xsd;nonNegativeInteger">1</owl:maxQualifiedCardinality>
                        <owl:onDataRange rdf:resource="&xsd;float"/>
                    </owl:Restriction>
                </owl:intersectionOf>
            </owl:Class>
        </owl:equivalentClass>
        <rdfs:comment>A match that is reported by a Taxonomic Name Resolution Service (TNRS) for a submitted name.</rdfs:comment>
    </owl:Class>
    


    <!-- http://phylotastic.org/terms/tnrs.rdf#NameResolution -->

    <owl:Class rdf:about="http://phylotastic.org/terms/tnrs.rdf#NameResolution">
        <rdfs:label>Name resolution</rdfs:label>
        <owl:equivalentClass>
            <owl:Class>
                <owl:intersectionOf rdf:parseType="Collection">
                    <owl:Restriction>
                        <owl:onProperty rdf:resource="http://phylotastic.org/terms/tnrs.rdf#matches"/>
                        <owl:onClass rdf:resource="http://phylotastic.org/terms/tnrs.rdf#Match"/>
                        <owl:minQualifiedCardinality rdf:datatype="&xsd;nonNegativeInteger">0</owl:minQualifiedCardinality>
                    </owl:Restriction>
                    <owl:Restriction>
                        <owl:onProperty rdf:resource="http://phylotastic.org/terms/tnrs.rdf#matchCount"/>
                        <owl:qualifiedCardinality rdf:datatype="&xsd;nonNegativeInteger">1</owl:qualifiedCardinality>
                        <owl:onDataRange rdf:resource="&xsd;integer"/>
                    </owl:Restriction>
                    <owl:Restriction>
                        <owl:onProperty rdf:resource="http://phylotastic.org/terms/tnrs.rdf#submittedName"/>
                        <owl:qualifiedCardinality rdf:datatype="&xsd;nonNegativeInteger">1</owl:qualifiedCardinality>
                        <owl:onDataRange rdf:resource="&xsd;string"/>
                    </owl:Restriction>
                </owl:intersectionOf>
            </owl:Class>
        </owl:equivalentClass>
        <rdfs:comment>The result of a Taxonomic Name Resolution Servivce (TNRS) request.</rdfs:comment>
    </owl:Class>
    


    <!-- http://phylotastic.org/terms/tnrs.rdf#ResolutionRequest -->

    <owl:Class rdf:about="http://phylotastic.org/terms/tnrs.rdf#ResolutionRequest">
        <rdfs:label>Resolution request</rdfs:label>
        <owl:equivalentClass>
            <owl:Class>
                <owl:intersectionOf rdf:parseType="Collection">
                    <owl:Restriction>
                        <owl:onProperty rdf:resource="http://phylotastic.org/terms/tnrs.rdf#usedSource"/>
                        <owl:someValuesFrom rdf:resource="http://phylotastic.org/terms/tnrs.rdf#ResolutionSource"/>
                    </owl:Restriction>
                    <owl:Restriction>
                        <owl:onProperty rdf:resource="http://phylotastic.org/terms/tnrs.rdf#submitDate"/>
                        <owl:qualifiedCardinality rdf:datatype="&xsd;nonNegativeInteger">1</owl:qualifiedCardinality>
                        <owl:onDataRange rdf:resource="&xsd;dateTime"/>
                    </owl:Restriction>
                </owl:intersectionOf>
            </owl:Class>
        </owl:equivalentClass>
        <rdfs:comment>A taxonomic name resolution request to a Taxonomic Name Resolution Service (TNRS).</rdfs:comment>
    </owl:Class>
    


    <!-- http://phylotastic.org/terms/tnrs.rdf#ResolutionSource -->

    <owl:Class rdf:about="http://phylotastic.org/terms/tnrs.rdf#ResolutionSource">
        <rdfs:label>Resolution source</rdfs:label>
        <owl:equivalentClass>
            <owl:Class>
                <owl:intersectionOf rdf:parseType="Collection">
                    <owl:Restriction>
                        <owl:onProperty rdf:resource="http://phylotastic.org/terms/tnrs.rdf#hasRank"/>
                        <owl:maxQualifiedCardinality rdf:datatype="&xsd;nonNegativeInteger">1</owl:maxQualifiedCardinality>
                        <owl:onDataRange rdf:resource="&xsd;nonNegativeInteger"/>
                    </owl:Restriction>
                    <owl:Restriction>
                        <owl:onProperty rdf:resource="http://phylotastic.org/terms/tnrs.rdf#sourceStatus"/>
                        <owl:maxQualifiedCardinality rdf:datatype="&xsd;nonNegativeInteger">1</owl:maxQualifiedCardinality>
                        <owl:onDataRange rdf:resource="&xsd;string"/>
                    </owl:Restriction>
                    <owl:Restriction>
                        <owl:onProperty rdf:resource="&dc;title"/>
                        <owl:maxQualifiedCardinality rdf:datatype="&xsd;nonNegativeInteger">1</owl:maxQualifiedCardinality>
                        <owl:onDataRange rdf:resource="&xsd;string"/>
                    </owl:Restriction>
                </owl:intersectionOf>
            </owl:Class>
        </owl:equivalentClass>
        <rdfs:comment>A source used by a Taxonomic Name Resolution Service (TNRS).</rdfs:comment>
    </owl:Class>
    


    <!-- http://purl.obolibrary.org/obo/CDAO_0000138 -->

    <owl:Class rdf:about="&obo;CDAO_0000138">
        <rdfs:label>TU</rdfs:label>
    </owl:Class>
</rdf:RDF>



<!-- Generated by the OWL API (version 3.3.1957) http://owlapi.sourceforge.net -->

