<?xml version="1.0"?>


<!DOCTYPE rdf:RDF [
    <!ENTITY owl "http://www.w3.org/2002/07/owl#" >
    <!ENTITY xsd "http://www.w3.org/2001/XMLSchema#" >
    <!ENTITY rdfs "http://www.w3.org/2000/01/rdf-schema#" >
    <!ENTITY tnrs "http://phylotastic.org/terms/tnrs.rdf#" >
    <!ENTITY rdf "http://www.w3.org/1999/02/22-rdf-syntax-ns#" >
]>


<rdf:RDF xmlns="http://phylotastic.org/terms/tnrs.rdf#"
     xml:base="http://phylotastic.org/terms/tnrs.rdf"
     xmlns:tnrs="http://phylotastic.org/terms/tnrs.rdf#"
     xmlns:rdfs="http://www.w3.org/2000/01/rdf-schema#"
     xmlns:owl="http://www.w3.org/2002/07/owl#"
     xmlns:xsd="http://www.w3.org/2001/XMLSchema#"
     xmlns:rdf="http://www.w3.org/1999/02/22-rdf-syntax-ns#">
    <owl:Ontology rdf:about="http://phylotastic.org/terms/tnrs.rdf">
        <owl:versionIRI rdf:resource="http://phylotastic.org/terms/2012-06-08/tnrs.rdf"/>
    </owl:Ontology>
    


    <!-- 
    ///////////////////////////////////////////////////////////////////////////////////////
    //
    // Annotation properties
    //
    ///////////////////////////////////////////////////////////////////////////////////////
     -->

    


    <!-- 
    ///////////////////////////////////////////////////////////////////////////////////////
    //
    // Datatypes
    //
    ///////////////////////////////////////////////////////////////////////////////////////
     -->

    


    <!-- 
    ///////////////////////////////////////////////////////////////////////////////////////
    //
    // Object Properties
    //
    ///////////////////////////////////////////////////////////////////////////////////////
     -->

    


    <!-- http://phylotastic.org/terms/tnrs.rdf#matches -->

    <owl:ObjectProperty rdf:about="&tnrs;matches">
        <rdfs:label>matches</rdfs:label>
        <rdfs:comment>The relationship between a taxonomic name resolution request for a name and the resulting matches.</rdfs:comment>
        <rdfs:range rdf:resource="&tnrs;Match"/>
        <rdfs:domain rdf:resource="&tnrs;NameResolution"/>
    </owl:ObjectProperty>
    


    <!-- http://phylotastic.org/terms/tnrs.rdf#resolvesAs -->

    <owl:ObjectProperty rdf:about="&tnrs;resolvesAs">
        <rdfs:label>resolvesAs</rdfs:label>
        <rdfs:comment>The relationship between a taxonomic unit or entity and its taxonomic name resolution.</rdfs:comment>
        <rdfs:range rdf:resource="&tnrs;NameResolution"/>
    </owl:ObjectProperty>
    


    <!-- http://phylotastic.org/terms/tnrs.rdf#usedSource -->

    <owl:ObjectProperty rdf:about="&tnrs;usedSource">
        <rdfs:label>usedSource</rdfs:label>
        <rdfs:comment>The relationship between a TNRS resolution request and the resolution sources used by the TNRS in carrying out the request.</rdfs:comment>
        <rdfs:domain rdf:resource="&tnrs;ResolutionRequest"/>
        <rdfs:range rdf:resource="&tnrs;ResolutionSource"/>
    </owl:ObjectProperty>
    


    <!-- 
    ///////////////////////////////////////////////////////////////////////////////////////
    //
    // Data properties
    //
    ///////////////////////////////////////////////////////////////////////////////////////
     -->

    


    <!-- http://phylotastic.org/terms/tnrs.rdf#acceptedName -->

    <owl:DatatypeProperty rdf:about="&tnrs;acceptedName">
        <rdfs:label>acceptedName</rdfs:label>
        <rdfs:comment>The taxonomic name reported as accepted name by the TNRS source reporting a match to a query.</rdfs:comment>
    </owl:DatatypeProperty>
    


    <!-- http://phylotastic.org/terms/tnrs.rdf#hasRank -->

    <owl:DatatypeProperty rdf:about="&tnrs;hasRank">
        <rdfs:label>hasRank</rdfs:label>
        <rdfs:comment>The suggested rank of a TNRS source among the sources a TNRS queries.</rdfs:comment>
    </owl:DatatypeProperty>
    


    <!-- http://phylotastic.org/terms/tnrs.rdf#hasURI -->

    <owl:DatatypeProperty rdf:about="&tnrs;hasURI">
        <rdf:type rdf:resource="&owl;FunctionalProperty"/>
        <rdfs:label>hasURI</rdfs:label>
        <rdfs:comment>The URI for a TNRS entity, such as the URI for a TNRS source, or for the accepted name reported by a TNRS source. URIs are unique, i.e., two entities with the same value of this property are the same.</rdfs:comment>
    </owl:DatatypeProperty>
    


    <!-- http://phylotastic.org/terms/tnrs.rdf#matchCount -->

    <owl:DatatypeProperty rdf:about="&tnrs;matchCount">
        <rdfs:label>matchCount</rdfs:label>
        <rdfs:comment>The number of matches obtained from the TNRS query for a submitted name.</rdfs:comment>
    </owl:DatatypeProperty>
    


    <!-- http://phylotastic.org/terms/tnrs.rdf#matchedName -->

    <owl:DatatypeProperty rdf:about="&tnrs;matchedName">
        <rdfs:label>matchedName</rdfs:label>
        <rdfs:comment>The taxonomic name matched by a TNRS source.</rdfs:comment>
    </owl:DatatypeProperty>
    


    <!-- http://phylotastic.org/terms/tnrs.rdf#score -->

    <owl:DatatypeProperty rdf:about="&tnrs;score">
        <rdfs:label>score</rdfs:label>
        <rdfs:comment>The score of a match reported by a TNRS source.</rdfs:comment>
    </owl:DatatypeProperty>
    


    <!-- http://phylotastic.org/terms/tnrs.rdf#sourceId -->

    <owl:DatatypeProperty rdf:about="&tnrs;sourceId">
        <rdf:type rdf:resource="&owl;FunctionalProperty"/>
        <rdfs:label>sourceId</rdfs:label>
        <rdfs:comment>The ID of a source queried by a TNRS. TNRS source IDs need to be unique.</rdfs:comment>
    </owl:DatatypeProperty>
    


    <!-- http://phylotastic.org/terms/tnrs.rdf#sourceName -->

    <owl:DatatypeProperty rdf:about="&tnrs;sourceName">
        <rdfs:label>sourceName</rdfs:label>
        <rdfs:comment>The name under which a TNRS source is commonly known.</rdfs:comment>
    </owl:DatatypeProperty>
    


    <!-- http://phylotastic.org/terms/tnrs.rdf#sourceStatus -->

    <owl:DatatypeProperty rdf:about="&tnrs;sourceStatus">
        <rdfs:label>sourceStatus</rdfs:label>
        <rdfs:comment>The status of a TNRS source at the time the request was made. TNRS sources with &quot;offline&quot; or &quot;temporarily offline&quot; status may NOT have been queried, and their results may be missing from the resolution document.</rdfs:comment>
    </owl:DatatypeProperty>
    


    <!-- http://phylotastic.org/terms/tnrs.rdf#submitDate -->

    <owl:DatatypeProperty rdf:about="&tnrs;submitDate">
        <rdfs:label>submitDate</rdfs:label>
        <rdfs:comment>The date and time that the TNRS resolution job was submitted, in ISO 8601 format.</rdfs:comment>
    </owl:DatatypeProperty>
    


    <!-- http://phylotastic.org/terms/tnrs.rdf#submittedName -->

    <owl:DatatypeProperty rdf:about="&tnrs;submittedName">
        <rdfs:label>submittedName</rdfs:label>
        <rdfs:comment>The name that was submitted to the TNRS for resolution.</rdfs:comment>
    </owl:DatatypeProperty>
    


    <!-- 
    ///////////////////////////////////////////////////////////////////////////////////////
    //
    // Classes
    //
    ///////////////////////////////////////////////////////////////////////////////////////
     -->

    


    <!-- http://phylotastic.org/terms/tnrs.rdf#Match -->

    <owl:Class rdf:about="&tnrs;Match">
        <rdfs:label>Match</rdfs:label>
        <owl:equivalentClass>
            <owl:Class>
                <owl:intersectionOf rdf:parseType="Collection">
                    <owl:Restriction>
                        <owl:onProperty rdf:resource="&tnrs;acceptedName"/>
                        <owl:qualifiedCardinality rdf:datatype="&xsd;nonNegativeInteger">1</owl:qualifiedCardinality>
                        <owl:onDataRange rdf:resource="&xsd;string"/>
                    </owl:Restriction>
                    <owl:Restriction>
                        <owl:onProperty rdf:resource="&tnrs;hasURI"/>
                        <owl:qualifiedCardinality rdf:datatype="&xsd;nonNegativeInteger">1</owl:qualifiedCardinality>
                        <owl:onDataRange rdf:resource="&xsd;anyURI"/>
                    </owl:Restriction>
                    <owl:Restriction>
                        <owl:onProperty rdf:resource="&tnrs;matchedName"/>
                        <owl:qualifiedCardinality rdf:datatype="&xsd;nonNegativeInteger">1</owl:qualifiedCardinality>
                        <owl:onDataRange rdf:resource="&xsd;string"/>
                    </owl:Restriction>
                    <owl:Restriction>
                        <owl:onProperty rdf:resource="&tnrs;sourceId"/>
                        <owl:qualifiedCardinality rdf:datatype="&xsd;nonNegativeInteger">1</owl:qualifiedCardinality>
                        <owl:onDataRange rdf:resource="&xsd;NMTOKEN"/>
                    </owl:Restriction>
                    <owl:Restriction>
                        <owl:onProperty rdf:resource="&tnrs;score"/>
                        <owl:maxQualifiedCardinality rdf:datatype="&xsd;nonNegativeInteger">1</owl:maxQualifiedCardinality>
                        <owl:onDataRange rdf:resource="&xsd;float"/>
                    </owl:Restriction>
                </owl:intersectionOf>
            </owl:Class>
        </owl:equivalentClass>
        <rdfs:comment>A match that is reported by a Taxonomic Name Resolution Service (TNRS) for a submitted name.</rdfs:comment>
    </owl:Class>
    


    <!-- http://phylotastic.org/terms/tnrs.rdf#NameResolution -->

    <owl:Class rdf:about="&tnrs;NameResolution">
        <rdfs:label>Name resolution</rdfs:label>
        <owl:equivalentClass>
            <owl:Class>
                <owl:intersectionOf rdf:parseType="Collection">
                    <owl:Restriction>
                        <owl:onProperty rdf:resource="&tnrs;matches"/>
                        <owl:onClass rdf:resource="&tnrs;Match"/>
                        <owl:minQualifiedCardinality rdf:datatype="&xsd;nonNegativeInteger">0</owl:minQualifiedCardinality>
                    </owl:Restriction>
                    <owl:Restriction>
                        <owl:onProperty rdf:resource="&tnrs;matchCount"/>
                        <owl:qualifiedCardinality rdf:datatype="&xsd;nonNegativeInteger">1</owl:qualifiedCardinality>
                        <owl:onDataRange rdf:resource="&xsd;integer"/>
                    </owl:Restriction>
                    <owl:Restriction>
                        <owl:onProperty rdf:resource="&tnrs;submittedName"/>
                        <owl:qualifiedCardinality rdf:datatype="&xsd;nonNegativeInteger">1</owl:qualifiedCardinality>
                        <owl:onDataRange rdf:resource="&xsd;string"/>
                    </owl:Restriction>
                </owl:intersectionOf>
            </owl:Class>
        </owl:equivalentClass>
        <rdfs:comment>The result of a Taxonomic Name Resolution Servivce (TNRS) request.</rdfs:comment>
    </owl:Class>
    


    <!-- http://phylotastic.org/terms/tnrs.rdf#ResolutionRequest -->

    <owl:Class rdf:about="&tnrs;ResolutionRequest">
        <rdfs:label>Resolution request</rdfs:label>
        <owl:equivalentClass>
            <owl:Class>
                <owl:intersectionOf rdf:parseType="Collection">
                    <owl:Restriction>
                        <owl:onProperty rdf:resource="&tnrs;usedSource"/>
                        <owl:someValuesFrom rdf:resource="&tnrs;ResolutionSource"/>
                    </owl:Restriction>
                    <owl:Restriction>
                        <owl:onProperty rdf:resource="&tnrs;submitDate"/>
                        <owl:maxQualifiedCardinality rdf:datatype="&xsd;nonNegativeInteger">1</owl:maxQualifiedCardinality>
                        <owl:onDataRange rdf:resource="&xsd;dateTime"/>
                    </owl:Restriction>
                </owl:intersectionOf>
            </owl:Class>
        </owl:equivalentClass>
        <rdfs:comment>A taxonomic name resolution request to a Taxonomic Name Resolution Service (TNRS).</rdfs:comment>
    </owl:Class>
    


    <!-- http://phylotastic.org/terms/tnrs.rdf#ResolutionSource -->

    <owl:Class rdf:about="&tnrs;ResolutionSource">
        <rdfs:label>Resolution source</rdfs:label>
        <rdfs:subClassOf>
            <owl:Restriction>
                <owl:onProperty rdf:resource="&tnrs;sourceName"/>
                <owl:maxQualifiedCardinality rdf:datatype="&xsd;nonNegativeInteger">1</owl:maxQualifiedCardinality>
                <owl:onDataRange rdf:resource="&xsd;string"/>
            </owl:Restriction>
        </rdfs:subClassOf>
        <rdfs:subClassOf>
            <owl:Restriction>
                <owl:onProperty rdf:resource="&tnrs;hasURI"/>
                <owl:maxQualifiedCardinality rdf:datatype="&xsd;nonNegativeInteger">1</owl:maxQualifiedCardinality>
                <owl:onDataRange rdf:resource="&xsd;anyURI"/>
            </owl:Restriction>
        </rdfs:subClassOf>
        <rdfs:subClassOf>
            <owl:Restriction>
                <owl:onProperty rdf:resource="&tnrs;sourceStatus"/>
                <owl:maxQualifiedCardinality rdf:datatype="&xsd;nonNegativeInteger">1</owl:maxQualifiedCardinality>
                <owl:onDataRange rdf:resource="&xsd;string"/>
            </owl:Restriction>
        </rdfs:subClassOf>
        <rdfs:subClassOf>
            <owl:Restriction>
                <owl:onProperty rdf:resource="&tnrs;sourceId"/>
                <owl:someValuesFrom rdf:resource="&xsd;NMTOKEN"/>
            </owl:Restriction>
        </rdfs:subClassOf>
        <rdfs:subClassOf>
            <owl:Restriction>
                <owl:onProperty rdf:resource="&tnrs;hasRank"/>
                <owl:maxQualifiedCardinality rdf:datatype="&xsd;nonNegativeInteger">1</owl:maxQualifiedCardinality>
                <owl:onDataRange rdf:resource="&xsd;nonNegativeInteger"/>
            </owl:Restriction>
        </rdfs:subClassOf>
        <rdfs:comment>A source used by a Taxonomic Name Resolution Service (TNRS).</rdfs:comment>
    </owl:Class>
</rdf:RDF>



<!-- Generated by the OWL API (version 3.2.3.1824) http://owlapi.sourceforge.net -->

